tests/Groups.v
@@ -1,906 +1,402 @@
 
-Require Import MirrorSolve.SMT.
-Require Import MirrorSolve.BV.
-
-(* pulled from: https://people.cs.umass.edu/~arjun/courses/cs691pl-spring2014/assignments/groups.html *)
-
-(* The set of the group. *)
-(*** MS BEGIN {"type": "definition"} *)
-Parameter G : Set.
-(*** MS END {"type": "definition"} *)
-
-(* The binary operator. *)
-(*** MS BEGIN {"type": "definition"} *)
-Parameter f : G -> G -> G.
-(*** MS END {"type": "definition"} *)
-
-(* The group identity. *)
-(*** MS BEGIN {"type": "definition"} *)
-Parameter e : G.
-(*** MS END {"type": "definition"} *)
-
-(* The inverse operator. *)
-(*** MS BEGIN {"type": "definition"} *)
-Parameter i : G -> G.
-(*** MS END {"type": "definition"} *)
-
-(* For readability, we use infix <+> to stand for the binary operator. *)
-Infix "<+>" := f (at level 50, left associativity).
-
-(* The operator [f] is associative. *)
-(*** MS BEGIN {"type": "definition"} *)
-Axiom assoc : forall a b c, a <+> b <+> c = a <+> (b <+> c).
-(*** MS END {"type": "definition"} *)
-
-(* [e] is the right-identity for all elements [a] *)
-(*** MS BEGIN {"type": "definition"} *)
-Axiom id_r : forall a, a <+> e = a.
-(*** MS END {"type": "definition"} *)
-
-(* [i a] is the right-inverse of [a]. *)
-(*** MS BEGIN {"type": "definition"} *)
-Axiom inv_r : forall a, a <+> i a = e.
-(*** MS END {"type": "definition"} *)
-
-(* encoding groups in in FOL *)
-
 Require Import MirrorSolve.FirstOrder.
-Require Import MirrorSolve.Groups.
 
-Require Import MirrorSolve.HLists.
-
+Require Import MirrorSolve.BV.
+Require Import MirrorSolve.SMT.
 Require Import MirrorSolve.UF.
-
-Require Import Coq.Strings.String.
-
-Require Import Coq.Lists.List.
-
-Import ListNotations.
-
-Set Universe Polymorphism.
-
-Notation sig := Groups.sig.
-
-Definition group_model := Groups.fm_model G e f i.
-
-Require Import MirrorSolve.HLists.
-
-Import HListNotations.
 
 Require Import MirrorSolve.Reflection.Core.
 Require Import MirrorSolve.Reflection.FM.
 Require Import MirrorSolve.Reflection.Tactics.
-
-(*** MS BEGIN {"type": "configuration", "config_type":"boilerplate"} *)
-MetaCoq Quote Definition t_f := f.
-MetaCoq Quote Definition t_i := i.
-MetaCoq Quote Definition t_e := e.
-(*** MS END {"type": "configuration", "config_type":"boilerplate"} *)
-
-(* Some match tactics for the meta-interpreter. 
-   The meta-interpreter converts these definitions into a reflection procedure between pure Coq goals and FOL terms in the UF + Groups combined theory. 
-*)
-
-(*** MS BEGIN {"type": "configuration", "config_type":"boilerplate"} *)
-Notation uf op := (tacFun _ _ (Mk_fun_sym sig _ _ op)).
-
-Definition match_tacs : list ((term -> bool) * tac_syn sig group_model) := [
-    ( eq_term t_f, uf f_f)
-  ; ( eq_term t_i, uf i_f )
-  ; ( eq_term t_e, uf e_f)
-  ].
-
-MetaCoq Quote Definition g_ind := (G).
-
-(* This is an analogous match but for reflecting Coq types into FOL sorts. *)
-Definition match_inds : list ((term -> bool) * Groups.sorts) := [
-    (eq_term g_ind, G')
-  ].
-(*** MS END {"type": "configuration", "config_type":"boilerplate"} *)
-
-
-Require Import Coq.Program.Equality.
-
-Lemma mt_wf: mtacs_wf sig group_model sorts_eq_dec match_tacs match_tacs.
-Proof.
-  unfold mtacs_wf, match_tacs.
-  unfold extract_denote_mtacs_rel_def, extract_denote_mtacs_some_inl_def, mtacs_extract_none_def;
-  intuition;
-  simpl.
-  - assert (t = t_f \/ t  = t_i \/ t = t_e) by shelve.
-    intuition;
-    subst.
-    + exfalso.
-      clear H.
-      unfold extract_t2rel in H0.
-      unfold extract_mtacs in H0.
-      simpl in H0.
-      unfold extract_fun in H0.
-      simpl in H0.
-      destruct (trim_prefix _); [congruence |].
-      destruct o; [|congruence].
-      destruct s;
-      destruct x.
-      vm_compute in H0.
-      destruct l; [congruence|];
-      destruct o; [|congruence].
-      destruct s;
-      destruct x.
-      destruct l; congruence.
-    + exfalso.
-      clear H.
-      unfold extract_t2rel in H0.
-      unfold extract_mtacs in H0.
-      simpl in H0.
-      unfold extract_fun in H0.
-      simpl in H0.
-      destruct (trim_prefix _); [congruence |].
-      destruct o; [|congruence].
-      destruct s;
-      destruct x.
-      vm_compute in H0.
-      destruct l; [congruence|];
-      destruct o; congruence.
-    + exfalso.
-      clear H.
-      unfold extract_t2rel in H0.
-      unfold extract_mtacs in H0.
-      simpl in H0.
-      unfold extract_fun in H0.
-      simpl in H0.
-      destruct (trim_prefix _); congruence.
-  - exfalso.
-    assert (t = t_f \/ t = t_i \/ t = t_e) by shelve.
-    intuition;
-    subst.
-    + unfold extract_t2rel in H0.
-      unfold extract_mtacs in H0.
-      simpl in H0.
-      unfold extract_fun in H0.
-      simpl in H0.
-      destruct (trim_prefix _); [congruence |].
-      destruct o; [|congruence].
-      destruct s;
-      destruct x.
-      vm_compute in H0.
-      destruct l; [congruence|];
-      destruct o; [|congruence].
-      destruct s;
-      destruct x.
-      destruct l; congruence.
-    + unfold extract_t2rel in H0.
-      unfold extract_mtacs in H0.
-      simpl in H0.
-      unfold extract_fun in H0.
-      simpl in H0.
-      destruct (trim_prefix _); [congruence |].
-      destruct o; [|congruence].
-      destruct s;
-      destruct x.
-      vm_compute in H0.
-      destruct l; [congruence|];
-      destruct o; congruence.
-    + unfold extract_t2rel in H0.
-      unfold extract_mtacs in H0.
-      simpl in H0.
-      unfold extract_fun in H0.
-      simpl in H0.
-      destruct (trim_prefix _); congruence.
-  - assert (tests = [(eq_term t_f, uf f_f); (eq_term t_i, uf i_f);
-  (eq_term t_e, uf e_f)]) by shelve.
-    subst.
-    pose proof trim_prefix_equiv_envs H.
-    assert (t = t_f \/ t = t_i \/ t = t_e) by shelve.
-    intuition;
-    subst.
-    * simpl in H1.
-      unfold extract_fun in H1.
-      destruct (trim_prefix er) eqn:?; [
-          simpl in H1; congruence
-        |
-      ].
-      destruct o; [|simpl in H1; congruence].
-      destruct s;
-      destruct x.
-      destruct l eqn:?; [simpl in H1; congruence|].
-      destruct o; [|simpl in H1; congruence].
-      destruct s;
-      destruct x.
-      destruct l0 eqn:?; [|simpl in H1; congruence].
-      simpl in H1.
-      inversion H1; subst.
-      do 3 dependent destruction H2.
-      unfold denote_mtacs.
-      unfold denote_mtac.
-      unfold denote_tac.
-      erewrite <- x0.
-      simpl.
-      unfold eq_rect_r; simpl eq_rect.
-      autorewrite with interp_tm.
-      simpl.
-      trivial.
-    * simpl in H1.
-      unfold extract_fun in H1.
-      destruct (trim_prefix er) eqn:?; [
-          simpl in H1; congruence
-        |
-      ].
-      destruct o; [|simpl in H1; congruence].
-      destruct s;
-      destruct x.
-      destruct l eqn:?; [|simpl in H1; congruence].
-      simpl in H1.
-      inversion H1; subst.
-      do 2 dependent destruction H2.
-      unfold denote_mtacs.
-      unfold denote_mtac.
-      unfold denote_tac.
-      erewrite <- x0.
-      simpl.
-      unfold eq_rect_r; simpl eq_rect.
-      autorewrite with interp_tm.
-      simpl.
-      trivial.
-    * simpl in H1.
-      unfold extract_fun in H1.
-      destruct (trim_prefix er) eqn:?; [
-        | simpl in H1; congruence
-      ].
-      simpl in H1.
-      inversion H1; subst.
-      dependent destruction H2.
-      unfold denote_mtacs.
-      unfold denote_mtac.
-      unfold denote_tac.
-      erewrite <- x.
-      simpl.
-      unfold eq_rect_r; simpl eq_rect.
-      autorewrite with interp_tm.
-      simpl.
-      trivial.
-  Unshelve.
-Admitted.
-
-
-(* Next we configure the backend solver. We need to tell the OCaml backend about: 
-   A custom sort symbol for the Groups.G' sort;
-   and custom UF symbols for e, op, and inv. 
-
-   The syntax for a UF declaration is 
-    RegisterSMTUF <symbol name as a string> <return sort> <list of argument sorts>
-*)
-(*** MS BEGIN {"type": "configuration", "config_type":"plugin"} *)
-Local Declare ML Module "mirrorsolve".
-RegisterCustomSort Groups.G' "G".
-RegisterSMTUF "e" G'.
-RegisterSMTUF "f" G' G' G'.
-RegisterSMTUF "i" G' G'.
-
-RegisterSMTFun Groups.e_f "e" 0.
-RegisterSMTFun Groups.f_f "f" 2.
-RegisterSMTFun Groups.i_f "i" 1.
-(*** MS END {"type": "configuration", "config_type":"plugin"} *)
-
-Transparent denote_tm.
-
-Require Import MirrorSolve.Axioms. (* trust the SMT solver in a typesafe way *)
-
-(*** MS BEGIN {"type": "configuration", "config_type":"tactics"} *)
-Ltac prep_proof := Utils.pose_all (tt, assoc, inv_r, id_r);
-  Utils.revert_all.
-
-Ltac extend_ctx H f := pose proof H;
-  f.
-
-Ltac reflect t := reflect_goal_trust sig group_model sorts_eq_dec match_tacs match_inds t.
- 
-
-Ltac check_goal := 
-  match goal with 
-  | |- ?G => check_unsat_neg G; eapply UnsoundAxioms.interp_true
-  end.
-
-SetSMTSolver "z3".
-(*** MS END {"type": "configuration", "config_type":"tactics"} *)
-
-(* Some group theory results translated into Coq *)
-
 From Hammer Require Import Hammer.
 
-Set Hammer ATPLimit 5.
-Set Hammer ReconstrLimit 10.
+Require Import MirrorSolve.Crush.
 
-MetaCoq Quote Definition unique_id_term := (
-  (forall a : G, a <+> e = a) ->
-(forall a : G, a <+> i a = e) ->
-(forall a b c : G, a <+> b <+> c = a <+> (b <+> c)) ->
-forall a : G, a <+> a = a -> a = e
-).
+Ltac hammer' := timeout 60 hammer.
+Ltac crush' := timeout 60 crush.
 
-(*** MS BEGIN {"type": "proof_definition"} *)
-Lemma unique_id : 
-  forall a, 
-    a <+> a = a -> 
-    a = e.
-(*** MS END {"type": "proof_definition"} *)
-Proof.
-  (*** MS BEGIN {"type": "proof", "proof_type":"manual"} *)
-  intros.
-  assert (a <+> i a = a <+> i a) by trivial.
-  erewrite <- H in H0 at 1.
-  erewrite assoc in H0.
-  erewrite inv_r in H0.
-  erewrite id_r in H0.
-  auto.
-  (*** MS END {"type": "proof", "proof_type":"manual"} *)
-  Restart.
-Proof.
-  (*** MS BEGIN {"type": "proof", "proof_type":"hammer", "total":1, "finished":1} *)
-  prep_proof;
-  hammer.
-  (*** MS END {"type": "proof", "proof_type":"hammer", "total":1, "finished":1} *)
-  Restart.
-Proof.
-  (*** MS BEGIN {"type": "proof", "proof_type":"mirrorsolve", "total":1} *)
-  prep_proof;
-  reflect unique_id_term;
-  check_goal.
-  (*** MS END {"type": "proof", "proof_type":"mirrorsolve", "total":1} *)
-Qed.
+Section Groups.
 
-Print Assumptions unique_id.
+  Unset Universe Polymorphism.
+  (* The set of the group. *)
+  (*** MS BEGIN {"type": "definition"} *)
+  Variable G : Set.
+  (*** MS END {"type": "definition"} *)
 
-(*** MS BEGIN {"type": "configuration", "config_type":"tactics"} *)
-Ltac prep_proof' := extend_ctx unique_id prep_proof.
-(*** MS END {"type": "configuration", "config_type":"tactics"} *)
+  (* The binary operator. *)
+  
+  (*** MS EFFORT {"type": "definition"} *)
+  (*** MS BEGIN {"type": "definition"} *)
+  Variable f : G -> G -> G.
+  Definition f' := f.
+  (*** MS END {"type": "definition"} *)
 
-(*** MS BEGIN {"type": "configuration", "config_type":"boilerplate"} *)
-MetaCoq Quote Definition inv_l_term := (
-  (forall a : G, a <+> a = a -> a = e) ->
-  (forall a : G, a <+> e = a) ->
-  (forall a : G, a <+> i a = e) ->
-  (forall a b c : G, a <+> b <+> c = a <+> (b <+> c)) ->
-  forall a : G, i a <+> a = e
-).
-(*** MS END {"type": "configuration", "config_type":"boilerplate"} *)
+  (* The group identity. *)
+  (*** MS EFFORT {"type": "definition"} *)
+  (*** MS BEGIN {"type": "definition"} *)
+  Variable e : G.
+  Definition e' := e.
+  (*** MS END {"type": "definition"} *)
 
-(* [i a] is the left-inverse of [a]. *)
-(*** MS BEGIN {"type": "proof_definition"} *)
-Lemma inv_l : 
-  forall a, 
-    i a <+> a = e.
-(*** MS END {"type": "proof_definition"} *)
-Proof.
-  (*** MS BEGIN {"type": "proof", "proof_type":"manual"} *)
-  intros.
-  eapply unique_id.
-  erewrite <- assoc.
-  erewrite assoc with (a := i a).
-  erewrite inv_r.
-  erewrite id_r.
-  trivial.
-  (*** MS END {"type": "proof", "proof_type":"manual"} *)
-  Restart.
-Proof.
-  (*** MS BEGIN {"type": "proof", "proof_type":"hammer", "total":1, "finished":1} *)
-  prep_proof';
-  hammer.
-  (*** MS END {"type": "proof", "proof_type":"hammer", "total":1, "finished":1} *)
-  Restart.
-Proof.
-  (*** MS BEGIN {"type": "proof", "proof_type":"mirrorsolve", "total":1} *)
-  prep_proof';
-  reflect inv_l_term;
-  check_goal.
-  (*** MS END {"type": "proof", "proof_type":"mirrorsolve", "total":1} *)
-Qed.
+  (* The inverse operator. *)
+  (*** MS EFFORT {"type": "definition"} *)
+  (*** MS BEGIN {"type": "definition"} *)
+  Variable i : G -> G.
+  Definition i' := i.
+  (*** MS END {"type": "definition"} *)
 
-Show Assumptions inv_l.
+  (* For readability, we use infix <+> to stand for the binary operator. *)
+  Infix "<+>" := f' (at level 50, left associativity).
+
+  (* The operator [f] is associative. *)
+  (*** MS EFFORT {"type": "edit"} *)
+  (*** MS BEGIN {"type": "definition"} *)
+  Axiom assoc : forall a b c, a <+> b <+> c = a <+> (b <+> c).
+  (*** MS END {"type": "definition"} *)
+
+  (* [e] is the right-identity for all elements [a] *)
+  (*** MS EFFORT {"type": "edit"} *)
+  (*** MS BEGIN {"type": "definition"} *)
+  Axiom id_r : forall a, a <+> e' = a.
+  (*** MS END {"type": "definition"} *)
+
+  (*** MS EFFORT {"type": "edit"} *)
+  (* [i a] is the right-inverse of [a]. *)
+  (*** MS BEGIN {"type": "definition"} *)
+  Axiom inv_r : forall a, a <+> i' a = e'.
+  (*** MS END {"type": "definition"} *)
+
+  (* encoding groups in in FOL *)
+
+  Local Declare ML Module "mirrorsolve".
+
+  From MetaCoq.Template Require Import All Loader.
+  Import MCMonadNotation.
+  Require Import MirrorSolve.Config.
+  Require Import Coq.Lists.List.
+  Import ListNotations.
+  Open Scope bs.
+
+  Universe foo.
+  MetaCoq Quote Definition typ_term := Type@{foo}.
+  
+  Notation pack x := (existT _ _ x).
+
+  Definition fun_syms : list Config.packed := ([
+      pack f'
+    ; pack e'
+    ; pack i'
+  ])%type.
+
+  Definition rel_syms : list Config.packed := ([ 
+  ])%type.
+
+  Definition prim_syms : list (Config.packed * String.string) := [
+  ].
+
+  MetaCoq Run (
+    xs <- add_funs typ_term fun_syms [] ;;
+    xs' <- tmQuote xs ;;
+    tmMkDefinition "trans_tbl" xs'
+  ).
+
+  MetaCoq Run (
+    gen_sig typ_term sorts fol_funs fol_rels 
+  ).
+  MetaCoq Run (
+    gen_interp_funs sorts interp_sorts fol_funs trans_tbl
+  ).
+  MetaCoq Run (
+    gen_interp_rels sorts interp_sorts fol_rels trans_tbl
+  ).
+  Definition fm_model := Build_model sig interp_sorts interp_funs interp_rels.
+  MetaCoq Run (
+    match Utils.find _ _ smt_fun_base_beq IntLit (Utils.flip trans_tbl.(mp_consts)) with 
+    | Some v => add_const_wf_instance sig fm_model v IntLit 
+    | None => tmReturn tt
+    end
+  ).
+  MetaCoq Run (
+    match Utils.find _ _ smt_fun_base_beq BoolLit (Utils.flip trans_tbl.(mp_consts)) with 
+    | Some v => add_const_wf_instance sig fm_model v BoolLit 
+    | None => tmReturn tt
+    end
+  ).
+  MetaCoq Run (
+    add_matches sig fm_model trans_tbl
+  ).
+  MetaCoq Run (
+    ctx <- build_printing_ctx sig sort_Prop trans_tbl prim_syms;; 
+    ctx' <- tmEval all ctx ;;
+    rhs <- tmQuote ctx' ;; 
+    tmMkDefinition "fol_theory" rhs
+  ).
+
+  Require Import MirrorSolve.Reflection.Tactics.
+
+  Transparent denote_tm.
+  Require Import MirrorSolve.Axioms.
+
+  (* We make use of the verification trick of negating the goal and checking for unsat. 
+    The check_unsat_neg tactic behaves like idtac if the negated goal is unsat and otherwise fails.
+    *)
+  Ltac check_goal_unsat := 
+    match goal with 
+    | |- ?G => check_unsat_neg_func fol_theory G; eapply UnsoundAxioms.interp_true
+    end.
+
+  Create HintDb groups_eqns.
+
+  Ltac prep_proof := 
+    hints_foreach (fun x => pose proof x) "groups_eqns";
+    Utils.revert_all;
+    unfold "<->" in *.
+
+  Scheme Equality for sorts.
+
+  Ltac quote_reflect_groups := quote_reflect sig fm_model sorts_eq_dec match_tacs match_sorts.
+
+  Ltac mirrorsolve :=
+    timeout 60 (prep_proof;
+    quote_reflect_groups;
+    check_goal_unsat).
+
+  SetSMTSolver "z3".
+  (*** MS END {"type": "configuration", "config_type":"tactics"} *)
 
 
-(*** MS BEGIN {"type": "configuration", "config_type":"tactics"} *)
-Ltac prep_proof'' := extend_ctx inv_l prep_proof'.
-(*** MS END {"type": "configuration", "config_type":"tactics"} *)
+  Hint Immediate assoc : groups_eqns.
+  Hint Immediate inv_r : groups_eqns.
+  Hint Immediate id_r : groups_eqns.
 
-(*** MS BEGIN {"type": "configuration", "config_type":"boilerplate"} *)
-MetaCoq Quote Definition id_l_term := (
-  (forall a : G, i a <+> a = e) ->
-  (forall a : G, a <+> a = a -> a = e) ->
-  (forall a : G, a <+> e = a) ->
-  (forall a : G, a <+> i a = e) ->
-  (forall a b c : G, a <+> b <+> c = a <+> (b <+> c)) ->
-  forall a : G, e <+> a = a
-).
-(*** MS END {"type": "configuration", "config_type":"boilerplate"} *)
+  (*** MS EFFORT {"type": "edit"} *)
+  (*** MS LEMMA {"original": True, "sfo": True, "tsfo": True, "ho": False, "goals": 1, "ms": 1, "hammer": 1, "crush": 0} *)
+  (*** MS BEGIN {"type": "proof_definition"} *)
+  Lemma unique_id : 
+    forall a, 
+      a <+> a = a -> 
+      a = e'.
+  (*** MS END {"type": "proof_definition"} *)
+  Proof.
+    try hammer'.
+    Restart.
+    try crush'.
+    Restart.
+    mirrorsolve.
+  Qed.
 
-(* [e] is the left-identity. *)
-(*** MS BEGIN {"type": "proof_definition"} *)
-Lemma id_l : 
-  forall a, 
-    e <+> a = a.
+  Hint Immediate unique_id : groups_eqns.
+
+  (* [i a] is the left-inverse of [a]. *)
+  (*** MS EFFORT {"type": "edit"} *)
+  (*** MS LEMMA {"original": True, "sfo": True, "tsfo": True, "ho": False, "goals": 1, "ms": 1, "hammer": 0, "crush": 0} *)
+  (*** MS BEGIN {"type": "proof_definition"} *)
+  Lemma inv_l : 
+    forall a, 
+      i' a <+> a = e'.
+  (*** MS END {"type": "proof_definition"} *)
+  Proof.
+    try hammer'.
+    Restart.
+    try crush'.
+    Restart.
+    mirrorsolve.
+  Qed.
+
+  Hint Immediate inv_l : groups_eqns.
+
+
+  (* [e] is the left-identity. *)
+  (*** MS EFFORT {"type": "edit"} *)
+  (*** MS LEMMA {"original": True, "sfo": True, "tsfo": True, "ho": False, "goals": 1, "ms": 1, "hammer": 1, "crush": 0} *)
+  (*** MS BEGIN {"type": "proof_definition"} *)
+  Lemma id_l : 
+    forall a, 
+      e' <+> a = a.
+      (*** MS END {"type": "proof_definition"} *)
+  Proof.
+    try hammer'.
+    Restart.
+    try crush'.
+    Restart.
+    mirrorsolve.
+  Qed.
+
+  Hint Immediate id_l : groups_eqns.
+
+
+  (* [x] can be cancelled on the right. *)
+  (*** MS LEMMA {"original": True, "sfo": True, "tsfo": True, "ho": False, "goals": 1, "ms": 0, "hammer": 0, "crush": 0} *)
+  (*** MS BEGIN {"type": "proof_definition"} *)
+  Lemma cancel_r : 
+    forall a b x, 
+      a <+> x = b <+> x -> 
+      a = b.
+      (*** MS END {"type": "proof_definition"} *)
+  Proof.
+    try hammer'.
+    Restart.
+    try crush'.
+    Restart.
+    SetSMTSolver "cvc5".
+    try mirrorsolve.
+  Admitted.
+
+  Hint Immediate cancel_r : groups_eqns.
+
+  (* [x] can be cancelled on the left. *)
+  (*** MS LEMMA {"original": True, "sfo": True, "tsfo": True, "ho": False, "goals": 1, "ms": 0, "hammer": 1, "crush": 0} *)
+  (*** MS BEGIN {"type": "proof_definition"} *)
+  Lemma cancel_l: 
+    forall a b x, 
+      x <+> a = x <+> b -> 
+      a = b.
     (*** MS END {"type": "proof_definition"} *)
-Proof.
-  (*** MS BEGIN {"type": "proof", "proof_type":"manual"} *)
-  intros.
-  erewrite <- inv_r with (a := a).
-  erewrite assoc.
-  erewrite inv_l.
-  erewrite id_r.
-  trivial.
-  (*** MS END {"type": "proof", "proof_type":"manual"} *)
-  Restart.
-Proof.
-  (*** MS BEGIN {"type": "proof", "proof_type":"hammer", "total":1, "finished":1} *)
-  prep_proof'';
-  hammer.
-  (*** MS END {"type": "proof", "proof_type":"hammer", "total":1, "finished":1} *)
-  Restart.
-Proof.
-  (*** MS BEGIN {"type": "proof", "proof_type":"mirrorsolve", "total":1} *)
-  prep_proof'';
-  reflect id_l_term;
-  check_goal.
-  (*** MS END {"type": "proof", "proof_type":"mirrorsolve", "total":1} *)
-Qed.
+  Proof.
+    try hammer'.
+    Restart.
+    try crush'.
+    Restart.
+    SetSMTSolver "z3".
+    try mirrorsolve.
+  Admitted.
 
+  Hint Immediate cancel_l : groups_eqns.
 
-(*** MS BEGIN {"type": "configuration", "config_type":"tactics"} *)
-Ltac prep_proof_0 := extend_ctx id_l prep_proof''.
-(*** MS END {"type": "configuration", "config_type":"tactics"} *)
-
-(*** MS BEGIN {"type": "configuration", "config_type":"boilerplate"} *)
-MetaCoq Quote Definition cancel_r_term := (
-  (forall a : G, e <+> a = a) ->
-  (forall a : G, i a <+> a = e) ->
-  (forall a : G, a <+> a = a -> a = e) ->
-  (forall a : G, a <+> e = a) ->
-  (forall a : G, a <+> i a = e) ->
-  (forall a b c : G, a <+> b <+> c = a <+> (b <+> c)) ->
-  forall a b x : G, a <+> x = b <+> x -> a = b
-).
-(*** MS END {"type": "configuration", "config_type":"boilerplate"} *)
-
-
-(* [x] can be cancelled on the right. *)
-(*** MS BEGIN {"type": "proof_definition"} *)
-Lemma cancel_r : 
-  forall a b x, 
-    a <+> x = b <+> x -> 
-    a = b.
+  (* The left identity is unique. *)
+  (*** MS EFFORT {"type": "edit"} *)
+  (*** MS LEMMA {"original": True, "sfo": True, "tsfo": True, "ho": False, "goals": 1, "ms": 1, "hammer": 1, "crush": 0} *)
+  (*** MS BEGIN {"type": "proof_definition"} *)
+  Lemma e_uniq_l : 
+    forall a p, 
+      p <+> a = a -> 
+      p = e'.
     (*** MS END {"type": "proof_definition"} *)
-Proof.
-  (*** MS BEGIN {"type": "proof", "proof_type":"manual"} *)
-  intros.
-  assert (a <+> x <+> i x = a <+> x <+> i x) by trivial.
-  erewrite H in H0 at 1.
-  repeat erewrite assoc in H0.
-  repeat erewrite inv_r in H0.
-  repeat erewrite id_r in H0.
-  auto.
-  (*** MS END {"type": "proof", "proof_type":"manual"} *)
-  Restart.
-Proof.
-  (*** MS BEGIN {"type": "proof", "proof_type":"hammer", "total":1, "finished":0} *)
-  (*
-  prep_proof_0;
-  hammer. *)
-  (*** MS END {"type": "proof", "proof_type":"hammer", "total":1, "finished":0} *)
-  Restart.
-Proof.
-  (*** MS BEGIN {"type": "proof", "proof_type":"mirrorsolve", "total":0} *)
-  (* prep_proof_0;
-  reflect cancel_r_term;
-  check_goal. *)
-  (*** MS END {"type": "proof", "proof_type":"mirrorsolve", "total":0} *)
-Admitted.
+  Proof. 
+    try hammer'.
+    Restart.
+    try crush'.
+    Restart.
+    try mirrorsolve.
+  Qed.
 
-(*** MS BEGIN {"type": "configuration", "config_type":"tactics"} *)
-Ltac prep_proof_1 := extend_ctx cancel_r prep_proof_0.
-(*** MS END {"type": "configuration", "config_type":"tactics"} *)
-
-(*** MS BEGIN {"type": "configuration", "config_type":"boilerplate"} *)
-MetaCoq Quote Definition cancel_l_term := (
-  (forall a b x : G, a <+> x = b <+> x -> a = b) ->
-  (forall a : G, e <+> a = a) ->
-  (forall a : G, i a <+> a = e) ->
-  (forall a : G, a <+> a = a -> a = e) ->
-  (forall a : G, a <+> e = a) ->
-  (forall a : G, a <+> i a = e) ->
-  (forall a b c : G, a <+> b <+> c = a <+> (b <+> c)) ->
-  forall a b x : G, x <+> a = x <+> b -> a = b
-).
-(*** MS END {"type": "configuration", "config_type":"boilerplate"} *)
-
-(* [x] can be cancelled on the left. *)
-(*** MS BEGIN {"type": "proof_definition"} *)
-Lemma cancel_l: 
-  forall a b x, 
-    x <+> a = x <+> b -> 
-    a = b.
-  (*** MS END {"type": "proof_definition"} *)
-Proof.
-  (*** MS BEGIN {"type": "proof", "proof_type":"manual"} *)
-  intros.
-  assert (i x <+> x <+> a = i x <+> x <+> a) by trivial.
-  erewrite assoc in H0.
-  erewrite H in H0 at 1.
-  repeat erewrite <- assoc in H0.
-  erewrite inv_l in H0.
-  repeat erewrite id_l in H0.
-  auto.
-  (*** MS END {"type": "proof", "proof_type":"manual"} *)
-  Restart.
-Proof.
-  (*** MS BEGIN {"type": "proof", "proof_type":"hammer", "total":1, "finished":0} *)
-  (* prep_proof_1; 
-  hammer. *)
-  (*** MS END {"type": "proof", "proof_type":"hammer", "total":1, "finished":0} *)
-  Restart.
-Proof.
-  (*** MS BEGIN {"type": "proof", "proof_type":"mirrorsolve", "total":0} *)
-  (* prep_proof_1;
-  reflect cancel_l_term;
-  check_goal. *)
-  (*** MS END {"type": "proof", "proof_type":"mirrorsolve", "total":0} *)
-Admitted.
-
-
-(*** MS BEGIN {"type": "configuration", "config_type":"tactics"} *)
-Ltac prep_proof_2 := extend_ctx cancel_l prep_proof_1.
-(*** MS END {"type": "configuration", "config_type":"tactics"} *)
-
-(*** MS BEGIN {"type": "configuration", "config_type":"boilerplate"} *)
-MetaCoq Quote Definition e_uniq_l_term := (
-  (forall a b x : G, x <+> a = x <+> b -> a = b) ->
-  (forall a b x : G, a <+> x = b <+> x -> a = b) ->
-  (forall a : G, e <+> a = a) ->
-  (forall a : G, i a <+> a = e) ->
-  (forall a : G, a <+> a = a -> a = e) ->
-  (forall a : G, a <+> e = a) ->
-  (forall a : G, a <+> i a = e) ->
-  (forall a b c : G, a <+> b <+> c = a <+> (b <+> c)) ->
-  forall a p : G, p <+> a = a -> p = e
-).
-(*** MS END {"type": "configuration", "config_type":"boilerplate"} *)
-
-(* The left identity is unique. *)
-(*** MS BEGIN {"type": "proof_definition"} *)
-Lemma e_uniq_l : 
-  forall a p, 
-    p <+> a = a -> 
-    p = e.
-  (*** MS END {"type": "proof_definition"} *)
-Proof. 
-  (*** MS BEGIN {"type": "proof", "proof_type":"manual"} *)
-  intros.
-  eapply cancel_r.
-  erewrite <- id_l in H.
-  eauto.
-  (*** MS END {"type": "proof", "proof_type":"manual"} *)
-  Restart.
-Proof.
-  (*** MS BEGIN {"type": "proof", "proof_type":"hammer", "total":1, "finished":1} *)
-  prep_proof_2;
-  hammer.
-  (*** MS END {"type": "proof", "proof_type":"hammer", "total":1, "finished":1} *)
-  Restart.
-Proof.
-  (*** MS BEGIN {"type": "proof", "proof_type":"mirrorsolve", "total":1} *)
-  prep_proof_2;
-  reflect e_uniq_l_term;
-  check_goal.
-  (*** MS END {"type": "proof", "proof_type":"mirrorsolve", "total":1} *)
-Qed.
-
-(*** MS BEGIN {"type": "configuration", "config_type":"tactics"} *)
-Ltac prep_proof_3 := extend_ctx e_uniq_l prep_proof_2.
-(*** MS END {"type": "configuration", "config_type":"tactics"} *)
-
-(*** MS BEGIN {"type": "configuration", "config_type":"boilerplate"} *)
-MetaCoq Quote Definition inv_uniq_l_term := (
-  (forall a p : G, p <+> a = a -> p = e) ->
-  (forall a b x : G, x <+> a = x <+> b -> a = b) ->
-  (forall a b x : G, a <+> x = b <+> x -> a = b) ->
-  (forall a : G, e <+> a = a) ->
-  (forall a : G, i a <+> a = e) ->
-  (forall a : G, a <+> a = a -> a = e) ->
-  (forall a : G, a <+> e = a) ->
-  (forall a : G, a <+> i a = e) ->
-  (forall a b c : G, a <+> b <+> c = a <+> (b <+> c)) ->
-  forall a b : G, a <+> b = e -> a = i b
-).
-(*** MS END {"type": "configuration", "config_type":"boilerplate"} *)
-
-(* The left inverse is unique. *)
-(*** MS BEGIN {"type": "proof_definition"} *)
-Lemma inv_uniq_l : 
-  forall a b, 
-    a <+> b = e -> 
-    a = i b.
-  (*** MS END {"type": "proof_definition"} *)
-Proof.
-  (*** MS BEGIN {"type": "proof", "proof_type":"manual"} *)
-  intros.
-  eapply cancel_r.
-  erewrite <- inv_l in H.
-  eauto.
-  (*** MS END {"type": "proof", "proof_type":"manual"} *)
-  Restart.
-Proof.
-  (*** MS BEGIN {"type": "proof", "proof_type":"hammer", "total":1, "finished":1} *)
-  prep_proof_3; 
-  hammer.
-  (*** MS END {"type": "proof", "proof_type":"hammer", "total":1, "finished":1} *)
-  Restart.
-Proof.
-  (*** MS BEGIN {"type": "proof", "proof_type":"mirrorsolve", "total":1} *)
-  prep_proof_3;
-  reflect inv_uniq_l_term;
-  check_goal.
-  (*** MS END {"type": "proof", "proof_type":"mirrorsolve", "total":1} *)
-Qed.
-
-(*** MS BEGIN {"type": "configuration", "config_type":"tactics"} *)
-Ltac prep_proof_4 := extend_ctx inv_uniq_l prep_proof_3.
-(*** MS END {"type": "configuration", "config_type":"tactics"} *)
-
-(*** MS BEGIN {"type": "configuration", "config_type":"boilerplate"} *)
-MetaCoq Quote Definition e_uniq_r_term := (
-  (forall a b : G, a <+> b = e -> a = i b) ->
-  (forall a p : G, p <+> a = a -> p = e) ->
-  (forall a b x : G, x <+> a = x <+> b -> a = b) ->
-  (forall a b x : G, a <+> x = b <+> x -> a = b) ->
-  (forall a : G, e <+> a = a) ->
-  (forall a : G, i a <+> a = e) ->
-  (forall a : G, a <+> a = a -> a = e) ->
-  (forall a : G, a <+> e = a) ->
-  (forall a : G, a <+> i a = e) ->
-  (forall a b c : G, a <+> b <+> c = a <+> (b <+> c)) ->
-  forall a p : G, a <+> p = a -> p = e
-).
-(*** MS END {"type": "configuration", "config_type":"boilerplate"} *)
-
-(* The right identity is unique. *)
-(*** MS BEGIN {"type": "proof_definition"} *)
-Lemma e_uniq_r : 
-  forall a p, 
-    a <+> p = a -> 
-    p = e.
-  (*** MS END {"type": "proof_definition"} *)
-Proof.
-  (*** MS BEGIN {"type": "proof", "proof_type":"manual"} *)
-  intros.
-  eapply cancel_l.
-  erewrite <- id_r in H.
-  eauto.
-  (*** MS END {"type": "proof", "proof_type":"manual"} *)
-  Restart.
-Proof.
-  (*** MS BEGIN {"type": "proof", "proof_type":"hammer", "total":1, "finished":1} *)
-  prep_proof_4; 
-  hammer.
-  (*** MS END {"type": "proof", "proof_type":"hammer", "total":1, "finished":1} *)
-  Restart.
-Proof.
-  (*** MS BEGIN {"type": "proof", "proof_type":"mirrorsolve", "total":1} *)
-  prep_proof_4;
-  reflect e_uniq_r_term;
-  check_goal.
-  (*** MS END {"type": "proof", "proof_type":"mirrorsolve", "total":1} *)
-Qed.
-
-
-(*** MS BEGIN {"type": "configuration", "config_type":"tactics"} *)
-Ltac prep_proof_5 := extend_ctx e_uniq_r prep_proof_4.
-(*** MS END {"type": "configuration", "config_type":"tactics"} *)
-
-(*** MS BEGIN {"type": "configuration", "config_type":"boilerplate"} *)
-MetaCoq Quote Definition inv_uniq_r_term := (
-  (forall a p : G, a <+> p = a -> p = e) ->
-(forall a b : G, a <+> b = e -> a = i b) ->
-(forall a p : G, p <+> a = a -> p = e) ->
-(forall a b x : G, x <+> a = x <+> b -> a = b) ->
-(forall a b x : G, a <+> x = b <+> x -> a = b) ->
-(forall a : G, e <+> a = a) ->
-(forall a : G, i a <+> a = e) ->
-(forall a : G, a <+> a = a -> a = e) ->
-(forall a : G, a <+> e = a) ->
-(forall a : G, a <+> i a = e) ->
-(forall a b c : G, a <+> b <+> c = a <+> (b <+> c)) ->
-forall a b : G, a <+> b = e -> b = i a
-).
-(*** MS END {"type": "configuration", "config_type":"boilerplate"} *)
-
-(* The right inverse is unique. *)
-(*** MS BEGIN {"type": "proof_definition"} *)
-Lemma inv_uniq_r : 
-  forall a b, 
-    a <+> b = e -> 
-    b = i a.
-  (*** MS END {"type": "proof_definition"} *)
-Proof.
-  (*** MS BEGIN {"type": "proof", "proof_type":"manual"} *)
-  intros.
-  eapply cancel_l.
-  erewrite <- inv_r in H.
-  eauto.
-  (*** MS END {"type": "proof", "proof_type":"manual"} *)
-  Restart.
-Proof.
-  (*** MS BEGIN {"type": "proof", "proof_type":"hammer", "total":1, "finished":1} *)
-  prep_proof_5; 
-  hammer.
-  (*** MS END {"type": "proof", "proof_type":"hammer", "total":1, "finished":1} *)
-  Restart.
-Proof.
-  (*** MS BEGIN {"type": "proof", "proof_type":"mirrorsolve", "total":1} *)
-  prep_proof_5.
-  reflect inv_uniq_r_term;
-  check_goal.
-  (*** MS END {"type": "proof", "proof_type":"mirrorsolve", "total":1} *)
-Qed.
-
-
-(*** MS BEGIN {"type": "configuration", "config_type":"tactics"} *)
-Ltac prep_proof_6 := extend_ctx inv_uniq_r prep_proof_5.
-(*** MS END {"type": "configuration", "config_type":"tactics"} *)
-
-(*** MS BEGIN {"type": "configuration", "config_type":"boilerplate"} *)
-MetaCoq Quote Definition inv_distr_term := (
-  (forall a b : G, a <+> b = e -> b = i a) ->
-(forall a p : G, a <+> p = a -> p = e) ->
-(forall a b : G, a <+> b = e -> a = i b) ->
-(forall a p : G, p <+> a = a -> p = e) ->
-(forall a b x : G, x <+> a = x <+> b -> a = b) ->
-(forall a b x : G, a <+> x = b <+> x -> a = b) ->
-(forall a : G, e <+> a = a) ->
-(forall a : G, i a <+> a = e) ->
-(forall a : G, a <+> a = a -> a = e) ->
-(forall a : G, a <+> e = a) ->
-(forall a : G, a <+> i a = e) ->
-(forall a b c : G, a <+> b <+> c = a <+> (b <+> c)) ->
-forall a b : G, i (a <+> b) = i b <+> i a
-).
-(*** MS END {"type": "configuration", "config_type":"boilerplate"} *)
-
-(* The right inverse is unique. *)
-
-(* The inverse operator distributes over the group operator. *)
-(*** MS BEGIN {"type": "proof_definition"} *)
-Lemma inv_distr : 
-  forall a b, 
-    i (a <+> b) = i b <+> i a.
+  (* The left inverse is unique. *)
+  (*** MS EFFORT {"type": "edit"} *)
+  (*** MS LEMMA {"original": True, "sfo": True, "tsfo": True, "ho": False, "goals": 1, "ms": 1, "hammer": 1, "crush": 0} *)
+  (*** MS BEGIN {"type": "proof_definition"} *)
+  Lemma inv_uniq_l : 
+    forall a b, 
+      a <+> b = e' -> 
+      a = i' b.
     (*** MS END {"type": "proof_definition"} *)
-Proof.
-  (*** MS BEGIN {"type": "proof", "proof_type":"manual"} *)
-  intros.
-  eapply eq_sym.
-  eapply inv_uniq_r.
-  erewrite <- assoc.
-  assert (a <+> b <+> i b <+> i a = a <+> (b <+> i b) <+> i a) by (now erewrite <- assoc).
-  erewrite H.
-  erewrite inv_r.
-  erewrite id_r.
-  eapply inv_r.
-  (*** MS END {"type": "proof", "proof_type":"manual"} *)
-  Restart.
-Proof.
-  (*** MS BEGIN {"type": "proof", "proof_type":"hammer", "total":1, "finished":1} *)
-  prep_proof_6; 
-  hammer.
-  (*** MS END {"type": "proof", "proof_type":"hammer", "total":1, "finished":1} *)
-  Restart.
-Proof.
-  (*** MS BEGIN {"type": "proof", "proof_type":"mirrorsolve", "total":1} *)
-  prep_proof_6.
-  reflect inv_distr_term;
-  check_goal.
-  (*** MS END {"type": "proof", "proof_type":"mirrorsolve", "total":1} *)
-Qed.
+  Proof.
+    (*** MS BEGIN {"type": "proof", "proof_type":"manual"} *)
+    intros.
+    eapply cancel_r.
+    erewrite <- inv_l in H.
+    eauto.
+    (*** MS END {"type": "proof", "proof_type":"manual"} *)
+    Restart.
+  Proof.
+    try hammer'.
+    Restart.
+    try crush'.
+    Restart.
+    try mirrorsolve.
+  Qed.
 
+  Hint Immediate inv_uniq_l : groups_eqns.
 
+  (* The right identity is unique. *)
+  (*** MS EFFORT {"type": "edit"} *)
+  (*** MS LEMMA {"original": True, "sfo": True, "tsfo": True, "ho": False, "goals": 1, "ms": 1, "hammer": 1, "crush": 0} *)
+  
+  (*** MS BEGIN {"type": "proof_definition"} *)
+  Lemma e_uniq_r : 
+    forall a p, 
+      a <+> p = a -> 
+      p = e'.
+    (*** MS END {"type": "proof_definition"} *)
+  Proof.
+    try hammer'.
+    Restart.
+    try crush'.
+    Restart.
+    try mirrorsolve.
+  Qed.
 
-(*** MS BEGIN {"type": "configuration", "config_type":"tactics"} *)
-Ltac prep_proof_7 := extend_ctx inv_distr prep_proof_6.
-(*** MS END {"type": "configuration", "config_type":"tactics"} *)
+  Hint Immediate e_uniq_r : groups_eqns.
 
-(*** MS BEGIN {"type": "configuration", "config_type":"boilerplate"} *)
-MetaCoq Quote Definition double_inv_term := (
-  (forall a b : G, i (a <+> b) = i b <+> i a) ->
-(forall a b : G, a <+> b = e -> b = i a) ->
-(forall a p : G, a <+> p = a -> p = e) ->
-(forall a b : G, a <+> b = e -> a = i b) ->
-(forall a p : G, p <+> a = a -> p = e) ->
-(forall a b x : G, x <+> a = x <+> b -> a = b) ->
-(forall a b x : G, a <+> x = b <+> x -> a = b) ->
-(forall a : G, e <+> a = a) ->
-(forall a : G, i a <+> a = e) ->
-(forall a : G, a <+> a = a -> a = e) ->
-(forall a : G, a <+> e = a) ->
-(forall a : G, a <+> i a = e) ->
-(forall a b c : G, a <+> b <+> c = a <+> (b <+> c)) ->
-forall a : G, i (i a) = a
-).
-(*** MS END {"type": "configuration", "config_type":"boilerplate"} *)
+  (* The right inverse is unique. *)
+  (*** MS EFFORT {"type": "edit"} *)
+  (*** MS LEMMA {"original": True, "sfo": True, "tsfo": True, "ho": False, "goals": 1, "ms": 1, "hammer": 1, "crush": 0} *)
+  
+  (*** MS BEGIN {"type": "proof_definition"} *)
+  Lemma inv_uniq_r : 
+    forall a b, 
+      a <+> b = e' -> 
+      b = i' a.
+    (*** MS END {"type": "proof_definition"} *)
+  Proof.
+    try hammer'.
+    Restart.
+    try crush'.
+    Restart.
+    SetSMTSolver "z3".
+    try mirrorsolve.
+  Qed.
 
+  Hint Immediate inv_uniq_r : groups_eqns.
 
-(* The inverse of an inverse produces the original element. *)
-(*** MS BEGIN {"type": "proof_definition"} *)
-Lemma double_inv : 
-  forall a, 
-    i (i a) = a.
-  (*** MS END {"type": "proof_definition"} *)
-Proof.
-  (*** MS BEGIN {"type": "proof", "proof_type":"manual"} *)
-  intros.
-  eapply eq_sym.
-  eapply inv_uniq_r.
-  eapply inv_l.
-  (*** MS END {"type": "proof", "proof_type":"manual"} *)
-  Restart.
-Proof.
-  (*** MS BEGIN {"type": "proof", "proof_type":"hammer", "total":1, "finished":1} *)
-  prep_proof_7; 
-  hammer.
-  (*** MS END {"type": "proof", "proof_type":"hammer", "total":1, "finished":1} *)
-  Restart.
-Proof.
-  (*** MS BEGIN {"type": "proof", "proof_type":"mirrorsolve", "total":1} *)
-  prep_proof_7.
-  reflect double_inv_term;
-  check_goal.
-  (*** MS END {"type": "proof", "proof_type":"mirrorsolve", "total":1} *)
-Qed.
+  (* The right inverse is unique. *)
 
+  (* The inverse operator distributes over the group operator. *)
+   (*** MS EFFORT {"type": "edit"} *)
+  (*** MS LEMMA {"original": True, "sfo": True, "tsfo": True, "ho": False, "goals": 1, "ms": 1, "hammer": 1, "crush": 0} *)
+  (*** MS BEGIN {"type": "proof_definition"} *)
+  Lemma inv_distr : 
+    forall a b, 
+      i' (a <+> b) = i' b <+> i' a.
+      (*** MS END {"type": "proof_definition"} *)
+  Proof.
+    try hammer'.
+    Restart.
+    try crush'.
+    Restart.
+    try mirrorsolve.
+  Qed.
 
-(*** MS BEGIN {"type": "configuration", "config_type":"tactics"} *)
-Ltac prep_proof_8 := extend_ctx inv_distr prep_proof_7.
-(*** MS END {"type": "configuration", "config_type":"tactics"} *)
+  (* The inverse of an inverse produces the original element. *)
+   (*** MS EFFORT {"type": "edit"} *)
+  (*** MS LEMMA {"original": True, "sfo": True, "tsfo": True, "ho": False, "goals": 1, "ms": 1, "hammer": 1, "crush": 0} *)
+  (*** MS BEGIN {"type": "proof_definition"} *)
+  Lemma double_inv : 
+    forall a, 
+      i' (i' a) = a.
+    (*** MS END {"type": "proof_definition"} *)
+  Proof.
+    try hammer'.
+    Restart.
+    try crush'.
+    Restart.
+    try mirrorsolve.
+  Qed.
 
-(*** MS BEGIN {"type": "configuration", "config_type":"boilerplate"} *)
-MetaCoq Quote Definition id_inv_term := (
-  (forall a b : G, i (a <+> b) = i b <+> i a) ->
-(forall a b : G, i (a <+> b) = i b <+> i a) ->
-(forall a b : G, a <+> b = e -> b = i a) ->
-(forall a p : G, a <+> p = a -> p = e) ->
-(forall a b : G, a <+> b = e -> a = i b) ->
-(forall a p : G, p <+> a = a -> p = e) ->
-(forall a b x : G, x <+> a = x <+> b -> a = b) ->
-(forall a b x : G, a <+> x = b <+> x -> a = b) ->
-(forall a : G, e <+> a = a) ->
-(forall a : G, i a <+> a = e) ->
-(forall a : G, a <+> a = a -> a = e) ->
-(forall a : G, a <+> e = a) ->
-(forall a : G, a <+> i a = e) ->
-(forall a b c : G, a <+> b <+> c = a <+> (b <+> c)) -> i e = e
-).
-(*** MS END {"type": "configuration", "config_type":"boilerplate"} *)
+  Hint Immediate double_inv : groups_eqns.
 
+  (* The identity is its own inverse. *)
+   (*** MS EFFORT {"type": "edit"} *)
+  (*** MS LEMMA {"original": True, "sfo": True, "tsfo": True, "ho": False, "goals": 1, "ms": 1, "hammer": 1, "crush": 0} *)
+  (*** MS BEGIN {"type": "proof_definition"} *)
+  Lemma id_inv : 
+    i' e' = e'.
+    (*** MS END {"type": "proof_definition"} *)
+  Proof.
+    try hammer'.
+    Restart.
+    try crush'.
+    Restart.
+    try mirrorsolve.
+  Qed.
 
-
-(* The identity is its own inverse. *)
-(*** MS BEGIN {"type": "proof_definition"} *)
-Lemma id_inv : 
-  i e = e.
-  (*** MS END {"type": "proof_definition"} *)
-Proof.
-  (*** MS BEGIN {"type": "proof", "proof_type":"manual"} *)
-  intros.
-  eapply eq_sym.
-  eapply inv_uniq_r.
-  eapply id_r.
-  (*** MS END {"type": "proof", "proof_type":"manual"} *)
-  Restart.
-Proof.
-  (*** MS BEGIN {"type": "proof", "proof_type":"hammer", "total":1, "finished":1} *)
-  prep_proof_8; 
-  hammer.
-  (*** MS END {"type": "proof", "proof_type":"hammer", "total":1, "finished":1} *)
-  Restart.
-Proof.
-  (*** MS BEGIN {"type": "proof", "proof_type":"mirrorsolve", "total":1} *)
-  prep_proof_8.
-  reflect id_inv_term;
-  check_goal.
-  (*** MS END {"type": "proof", "proof_type":"mirrorsolve", "total":1} *)
-Qed.
+End Groups.
